Lemma to initialize is_shard_server, fix ghost names

src/program_proof/memkv/memkv_shard_definitions.v
@@ -45,28 +45,28 @@ Record memkv_shard_names := {
 
 Implicit Type γ : memkv_shard_names.
 
-Definition PreShardGet Eo Ei γ key Q : iProp Σ :=
-  |={Eo,Ei}=> (∃ v, kvptsto γ.(kv_gn) key v ∗ (kvptsto γ.(kv_gn) key v -∗ |={Ei,Eo}=> Q v))
+Definition PreShardGet Eo Ei γkv key Q : iProp Σ :=
+  |={Eo,Ei}=> (∃ v, kvptsto γkv key v ∗ (kvptsto γkv key v -∗ |={Ei,Eo}=> Q v))
 .
 
-Definition PostShardGet Eo Ei γ (key:u64) Q (rep:ShardReplyC) : iProp Σ :=
-  ⌜rep.(SR_Err) ≠ 0⌝ ∗ (PreShardGet Eo Ei γ key Q) ∨ ⌜rep.(SR_Err) = 0⌝ ∗ (Q rep.(SR_Value)).
+Definition PostShardGet Eo Ei γkv (key:u64) Q (rep:ShardReplyC) : iProp Σ :=
+  ⌜rep.(SR_Err) ≠ 0⌝ ∗ (PreShardGet Eo Ei γkv key Q) ∨ ⌜rep.(SR_Err) = 0⌝ ∗ (Q rep.(SR_Value)).
 
-Definition PreShardPut Eo Ei γ key Q v : iProp Σ :=
-  |={Eo,Ei}=> (∃ oldv, kvptsto γ.(kv_gn) key oldv ∗ (kvptsto γ.(kv_gn) key v -∗ |={Ei,Eo}=> Q))
+Definition PreShardPut Eo Ei γkv key Q v : iProp Σ :=
+  |={Eo,Ei}=> (∃ oldv, kvptsto γkv key oldv ∗ (kvptsto γkv key v -∗ |={Ei,Eo}=> Q))
 .
 
-Definition PostShardPut Eo Ei γ (key:u64) Q v (rep:ShardReplyC) : iProp Σ :=
-  ⌜rep.(SR_Err) ≠ 0⌝ ∗ (PreShardPut Eo Ei γ key Q v) ∨ ⌜rep.(SR_Err) = 0⌝ ∗ Q .
+Definition PostShardPut Eo Ei γkv (key:u64) Q v (rep:ShardReplyC) : iProp Σ :=
+  ⌜rep.(SR_Err) ≠ 0⌝ ∗ (PreShardPut Eo Ei γkv key Q v) ∨ ⌜rep.(SR_Err) = 0⌝ ∗ Q .
 
-Definition PreShardConditionalPut Eo Ei γ key Q expv newv : iProp Σ :=
-  |={Eo,Ei}=> (∃ oldv, kvptsto γ.(kv_gn) key oldv ∗
-    (let succ := bool_decide (expv = oldv) in kvptsto γ.(kv_gn) key (if succ then newv else oldv) -∗
+Definition PreShardConditionalPut Eo Ei γkv key Q expv newv : iProp Σ :=
+  |={Eo,Ei}=> (∃ oldv, kvptsto γkv key oldv ∗
+    (let succ := bool_decide (expv = oldv) in kvptsto γkv key (if succ then newv else oldv) -∗
       |={Ei,Eo}=> Q succ))
 .
 
-Definition PostShardConditionalPut Eo Ei γ (key:u64) Q expv newv (rep:ShardReplyC) : iProp Σ :=
-  ⌜rep.(SR_Err) ≠ 0⌝ ∗ (PreShardConditionalPut Eo Ei γ key Q expv newv) ∨ ⌜rep.(SR_Err) = 0⌝ ∗ Q rep.(SR_Success).
+Definition PostShardConditionalPut Eo Ei γkv (key:u64) Q expv newv (rep:ShardReplyC) : iProp Σ :=
+  ⌜rep.(SR_Err) ≠ 0⌝ ∗ (PreShardConditionalPut Eo Ei γkv key Q expv newv) ∨ ⌜rep.(SR_Err) = 0⌝ ∗ Q rep.(SR_Success).
 
 
 Definition own_shard γkv sid (m:gmap u64 (list u8)) : iProp Σ :=
@@ -80,8 +80,8 @@ Definition is_shard_server_pre (ρ:u64 -d> memkv_shard_names -d> iPropO Σ) : (u
   "#HputSpec" ∷ handler_is (urpc_gn γ) (coPset * coPset * (iProp Σ) * rpc_request_names) host uKV_PUT
              (λ x reqData, ∃ req, ⌜has_encoding_PutRequest reqData req⌝ ∗
                   is_RPCRequest γ.(rpc_gn) x.2
-                     (PreShardPut x.1.1.1 x.1.1.2 γ req.(PR_Key) x.1.2 req.(PR_Value))
-                     (PostShardPut x.1.1.1 x.1.1.2 γ req.(PR_Key) x.1.2 req.(PR_Value))
+                     (PreShardPut x.1.1.1 x.1.1.2 γ.(kv_gn) req.(PR_Key) x.1.2 req.(PR_Value))
+                     (PostShardPut x.1.1.1 x.1.1.2 γ.(kv_gn) req.(PR_Key) x.1.2 req.(PR_Value))
                      {| Req_CID:=req.(PR_CID); Req_Seq:=req.(PR_Seq) |}
              ) (* pre *)
              (λ x reqData repData, ∃ req rep, ⌜has_encoding_PutReply repData rep⌝ ∗
@@ -93,8 +93,8 @@ Definition is_shard_server_pre (ρ:u64 -d> memkv_shard_names -d> iPropO Σ) : (u
   "#HconditionalPutSpec" ∷ handler_is (urpc_gn γ) (coPset * coPset * (bool → iProp Σ) * rpc_request_names) host uKV_CONDITIONAL_PUT
              (λ x reqData, ∃ req, ⌜has_encoding_ConditionalPutRequest reqData req⌝ ∗
                   is_RPCRequest γ.(rpc_gn) x.2
-                     (PreShardConditionalPut x.1.1.1 x.1.1.2 γ req.(CPR_Key) x.1.2 req.(CPR_ExpValue) req.(CPR_NewValue))
-                     (PostShardConditionalPut x.1.1.1 x.1.1.2 γ req.(CPR_Key) x.1.2 req.(CPR_ExpValue) req.(CPR_NewValue))
+                     (PreShardConditionalPut x.1.1.1 x.1.1.2 γ.(kv_gn) req.(CPR_Key) x.1.2 req.(CPR_ExpValue) req.(CPR_NewValue))
+                     (PostShardConditionalPut x.1.1.1 x.1.1.2 γ.(kv_gn) req.(CPR_Key) x.1.2 req.(CPR_ExpValue) req.(CPR_NewValue))
                      {| Req_CID:=req.(CPR_CID); Req_Seq:=req.(CPR_Seq) |}
              ) (* pre *)
              (λ x reqData repData, ∃ req rep, ⌜has_encoding_ConditionalPutReply repData rep⌝ ∗
@@ -105,8 +105,8 @@ Definition is_shard_server_pre (ρ:u64 -d> memkv_shard_names -d> iPropO Σ) : (u
 
   "#HgetSpec" ∷ handler_is (urpc_gn γ) (coPset * coPset * (list u8 → iProp Σ) * rpc_request_names) host uKV_GET
              (λ x reqData, ∃ req, ⌜has_encoding_GetRequest reqData req⌝ ∗
-                  is_RPCRequest γ.(rpc_gn) x.2 (PreShardGet x.1.1.1 x.1.1.2 γ req.(GR_Key) x.1.2)
-                    (PostShardGet x.1.1.1 x.1.1.2 γ req.(GR_Key) x.1.2)
+                  is_RPCRequest γ.(rpc_gn) x.2 (PreShardGet x.1.1.1 x.1.1.2 γ.(kv_gn) req.(GR_Key) x.1.2)
+                    (PostShardGet x.1.1.1 x.1.1.2 γ.(kv_gn) req.(GR_Key) x.1.2)
                     {| Req_CID:=req.(GR_CID); Req_Seq:=req.(GR_Seq) |}
              ) (* pre *)
              (λ x reqData repData, ∃ req rep, ⌜has_encoding_GetReply repData rep⌝ ∗
