src/program_proof/memkv/memkv_shard_ghost_init.v
@@ -1,0 +1,133 @@
+From Perennial.algebra Require Import gen_heap_names.
+From Perennial.goose_lang Require Import adequacy recovery_adequacy dist_adequacy.
+From Perennial.program_proof Require Import dist_prelude.
+From Goose.github_com.mit_pdos.gokv Require Import memkv.
+From Perennial.program_proof.lockservice Require Import rpc.
+
+From Perennial.program_proof.memkv Require Export memkv_shard_definitions.
+
+Section memkv_shard_ghost_init_proof.
+
+(* These lemmas happen *before* we get node local names (e.g. the gname for memory, crashes etc. *)
+Context `{!heapPreG Σ, !heap_globalG Σ, rpcG Σ ShardReplyC, rpcregG Σ, kvMapG Σ, invG Σ}.
+
+Let gn := heap_globalG_names.
+Let gpG := (heap_preG_ffi).
+
+Instance local_groveG : groveG Σ := {| groveG_gen_heapG := gen_heapG_update_pre (@grove_preG_gen_heapG _ gpG) gn |}.
+
+
+(* TODO: duplicating these specs is unfortunate, should try to unify with the set up in shard_definitions *)
+Definition is_shard_server_putSpec (γkv : gname) γrpc : RPCSpec :=
+  {| spec_rpcid := uKV_PUT;
+     spec_ty := (coPset * coPset * (iProp Σ) * rpc_request_names)%type;
+     spec_Pre := (λ x reqData, ∃ req, ⌜has_encoding_PutRequest reqData req⌝ ∗
+                  is_RPCRequest γrpc x.2
+                     (PreShardPut x.1.1.1 x.1.1.2 γkv req.(PR_Key) x.1.2 req.(PR_Value))
+                     (PostShardPut x.1.1.1 x.1.1.2 γkv req.(PR_Key) x.1.2 req.(PR_Value))
+                     {| Req_CID:=req.(PR_CID); Req_Seq:=req.(PR_Seq) |})%I;
+     spec_Post := (λ x reqData repData, ∃ req rep, ⌜has_encoding_PutReply repData rep⌝ ∗
+                  ⌜has_encoding_PutRequest reqData req⌝ ∗
+                  (RPCRequestStale γrpc {| Req_CID:=req.(PR_CID); Req_Seq:=req.(PR_Seq) |} ∨
+                    ∃ dummy_val dummy_succ, RPCReplyReceipt γrpc
+                                                            {| Req_CID:=req.(PR_CID); Req_Seq:=req.(PR_Seq) |}
+                                                            (mkShardReplyC rep.(PR_Err) dummy_val dummy_succ))
+             )%I |}.
+
+Definition is_shard_server_conditionalPutSpec γkv γrpc : RPCSpec :=
+  {| spec_rpcid := uKV_CONDITIONAL_PUT;
+     spec_ty := (coPset * coPset * (bool → iProp Σ) * rpc_request_names);
+     spec_Pre :=(λ x reqData, ∃ req, ⌜has_encoding_ConditionalPutRequest reqData req⌝ ∗
+                  is_RPCRequest γrpc x.2
+                     (PreShardConditionalPut x.1.1.1 x.1.1.2 γkv req.(CPR_Key) x.1.2 req.(CPR_ExpValue) req.(CPR_NewValue))
+                     (PostShardConditionalPut x.1.1.1 x.1.1.2 γkv req.(CPR_Key) x.1.2 req.(CPR_ExpValue) req.(CPR_NewValue))
+                     {| Req_CID:=req.(CPR_CID); Req_Seq:=req.(CPR_Seq) |}
+             )%I;
+     spec_Post :=(λ x reqData repData, ∃ req rep, ⌜has_encoding_ConditionalPutReply repData rep⌝ ∗
+                  ⌜has_encoding_ConditionalPutRequest reqData req⌝ ∗
+                  (RPCRequestStale γrpc {| Req_CID:=req.(CPR_CID); Req_Seq:=req.(CPR_Seq) |} ∨
+                    ∃ dummy_val, RPCReplyReceipt γrpc {| Req_CID:=req.(CPR_CID); Req_Seq:=req.(CPR_Seq) |} (mkShardReplyC rep.(CPR_Err) dummy_val rep.(CPR_Succ)))
+             )%I |}.
+
+Definition is_shard_server_getSpec γkv γrpc : RPCSpec :=
+  {| spec_rpcid := uKV_GET;
+     spec_ty := (coPset * coPset * (list u8 → iProp Σ) * rpc_request_names);
+     spec_Pre := (λ x reqData, ∃ req, ⌜has_encoding_GetRequest reqData req⌝ ∗
+                  is_RPCRequest γrpc x.2 (PreShardGet x.1.1.1 x.1.1.2 γkv req.(GR_Key) x.1.2)
+                    (PostShardGet x.1.1.1 x.1.1.2 γkv req.(GR_Key) x.1.2)
+                    {| Req_CID:=req.(GR_CID); Req_Seq:=req.(GR_Seq) |}
+             )%I;
+     spec_Post :=(λ x reqData repData, ∃ req rep, ⌜has_encoding_GetReply repData rep⌝ ∗
+                  ⌜has_encoding_GetRequest reqData req⌝ ∗
+                  (RPCRequestStale γrpc {| Req_CID:=req.(GR_CID); Req_Seq:=req.(GR_Seq) |} ∨
+                    ∃ dummy_succ, RPCReplyReceipt γrpc {| Req_CID:=req.(GR_CID); Req_Seq:=req.(GR_Seq) |} (mkShardReplyC rep.(GR_Err) rep.(GR_Value) dummy_succ))
+             )%I |}.
+
+Definition is_shard_server_moveSpec : @RPCSpec Σ :=
+  {| spec_rpcid := uKV_MOV_SHARD;
+     spec_ty := memkv_shard_names;
+     spec_Pre :=(λ x reqData, ∃ args, ⌜has_encoding_MoveShardRequest reqData args⌝ ∗
+                                  ⌜int.Z args.(MR_Sid) < uNSHARD⌝ ∗
+                                  (▷ is_shard_server args.(MR_Dst) x)
+             )%I;
+     spec_Post := (λ x reqData repData, True)%I |}.
+
+Definition is_shard_server_installSpec γkv γrpc : RPCSpec :=
+  {| spec_rpcid := uKV_INS_SHARD;
+     spec_ty := rpc_request_names;
+     spec_Pre := (λ x reqData, ∃ args, ⌜has_encoding_InstallShardRequest reqData args⌝ ∗
+                                  ⌜int.Z args.(IR_Sid) < uNSHARD⌝ ∗
+                                  is_RPCRequest γrpc x (own_shard γkv args.(IR_Sid) args.(IR_Kvs))
+                                                            (λ _, True)
+                                                            {| Req_CID:=args.(IR_CID); Req_Seq:=args.(IR_Seq) |}
+             )%I;
+     spec_Post := (λ x reqData repData, True)%I |}.
+
+Definition is_shard_server_freshSpec γrpc : RPCSpec :=
+  {| spec_rpcid := uKV_FRESHCID;
+     spec_ty := unit;
+     spec_Pre := (λ x reqData, True)%I;
+     spec_Post := (λ x reqData repData, ∃ cid, ⌜has_encoding_Uint64 repData cid⌝ ∗
+              RPCClient_own_ghost γrpc cid 1)%I |}.
+
+Definition shard_SpecList γkv γrpc : RPCSpecList :=
+  spec_cons (is_shard_server_putSpec γkv γrpc)
+    (spec_cons (is_shard_server_conditionalPutSpec γkv γrpc)
+      (spec_cons (is_shard_server_getSpec γkv γrpc)
+        (spec_cons (is_shard_server_moveSpec)
+          (spec_cons (is_shard_server_installSpec γkv γrpc)
+            (spec_cons (is_shard_server_freshSpec γrpc) spec_nil))))).
+
+Lemma shard_server_ghost_init host (γkv : gname) :
+  host c↦ ∅ ={⊤}=∗
+  ∃ γ, ⌜ γ.(kv_gn) = γkv ⌝ ∗
+       is_shard_server host γ ∗
+       RPCServer_own_ghost γ.(rpc_gn) ∅ ∅ ∗
+      ([∗ set] cid ∈ fin_to_set u64, RPCClient_own_ghost γ.(rpc_gn) cid 1).
+Proof.
+  iIntros "Hg".
+  iMod (make_rpc_server (R := ShardReplyC)) as (γrpc) "(#Hown&Hrpc1&Hrpc2)".
+  { set_solver. }
+  iMod (handler_is_init_list host (shard_SpecList γkv γrpc) with "[Hg]") as (γ) "H".
+  { simpl. set_solver. }
+  { iExactEq "Hg". f_equal. }
+  iDestruct "H" as "(#Hdom&#Hput&#Hcput&#Hget&#Hmove&#Hinstall&#Hfresh&_)".
+
+  set (Γsrv := {| rpc_gn := γrpc; urpc_gn := γ; kv_gn := γkv |}).
+  iAssert (is_shard_server host Γsrv) as "Hshard".
+  {
+    rewrite is_shard_server_unfold /is_shard_server_pre.
+    iSplitL.
+    { iFrame "#Hown". }
+    iSplitL. { iFrame "Hput". }
+    iSplitL. { iFrame "Hcput". }
+    iSplitL. { iFrame "Hget". }
+    iSplitL. { iFrame "Hmove". }
+    iSplitL. { iFrame "Hinstall". }
+    iFrame "Hfresh".
+  }
+  iExists Γsrv. iFrame "# ∗".
+  eauto.
+Qed.
+
+End memkv_shard_ghost_init_proof.
